Adding html extraction. Main change : literal -> (v p n) -> (L p n)

jSudoku.ml
@@ -1,0 +1,49 @@
+(* This program is free software; you can redistribute it and/or      *)
+(* modify it under the terms of the GNU Lesser General Public License *)
+(* as published by the Free Software Foundation; either version 2.1   *)
+(* of the License, or (at your option) any later version.             *)
+(*                                                                    *)
+(* This program is distributed in the hope that it will be useful,    *)
+(* but WITHOUT ANY WARRANTY; without even the implied warranty of     *)
+(* MERCHANTABILITY or FITNESS FOR A PARTICULAR PURPOSE.  See the      *)
+(* GNU General Public License for more details.                       *)
+(*                                                                    *)
+(* You should have received a copy of the GNU Lesser General Public   *)
+(* License along with this program; if not, write to the Free         *)
+(* Software Foundation, Inc., 51 Franklin St, Fifth Floor, Boston, MA *)
+(* 02110-1301 USA                                                     *)
+
+(** link code **)
+
+open Js_of_ocaml
+open Sudoku
+
+let rec n2nat n = if n = 0 then O else S (n2nat (n - 1))
+
+let rec nat2n n = match n with O -> 0 | S n -> 1 + (nat2n n)
+
+let string2l s =
+  let le = String.length s in
+  let rec iter i = if i = le then Nil else
+      Cons (n2nat (Char.code (String.get s i) - 48), iter (i + 1)) in
+  iter 0
+
+let rec l2stringr s l =
+  match l with
+    Nil -> s
+  | Cons (n,l) ->  l2stringr (s ^ (Char.escaped (Char.chr (nat2n n + 48)))) l
+
+let l2string l = l2stringr "" l
+
+let main s =
+  let l = string2l s in
+  match find_just_one (S (S (S O))) (S (S (S O))) l with
+  | JNone -> "N"
+  | JOne l -> "O" ^ (l2string l)
+  | JMore (l1,l2)  -> "M" ^ (l2string l1) ^ "M" ^ (l2string l2)
+
+let _ =
+  Js.export_all
+    (object%js
+      method solve s = Js.string (main (Js.to_string s))
+    end)
