Parse.v
@@ -1,0 +1,57 @@
+(* This program is free software; you can redistribute it and/or      *)
+(* modify it under the terms of the GNU Lesser General Public License *)
+(* as published by the Free Software Foundation; either version 2.1   *)
+(* of the License, or (at your option) any later version.             *)
+(*                                                                    *)
+(* This program is distributed in the hope that it will be useful,    *)
+(* but WITHOUT ANY WARRANTY; without even the implied warranty of     *)
+(* MERCHANTABILITY or FITNESS FOR A PARTICULAR PURPOSE.  See the      *)
+(* GNU General Public License for more details.                       *)
+(*                                                                    *)
+(* You should have received a copy of the GNU Lesser General Public   *)
+(* License along with this program; if not, write to the Free         *)
+(* Software Foundation, Inc., 51 Franklin St, Fifth Floor, Boston, MA *)
+(* 02110-1301 USA                                                     *)
+
+Require Import String.
+Import Ascii.
+Require Import List.
+Open Scope string_scope.
+Definition sp := 32.
+Definition nl := 10.
+Definition sep := 124.
+
+Fixpoint beq_nat (a b: nat) {struct a}: bool :=
+  match a, b with
+    S a1, S b1 => beq_nat a1 b1
+ | 0, 0 => true
+ | _,_ => false 
+  end.
+
+Definition is_num x := beq_nat ((48 - x) + (x - 57)) 0.
+Definition  get_num x :=  x - 48.
+
+Fixpoint mkline s acc {struct s} :=
+  match s with
+    String a s1 =>
+       let n := nat_of_ascii a in 
+       if beq_nat n sp then
+         match acc with 
+          Some x =>  mkline s1 (Some (0::x))
+        | _ => mkline s1 None
+         end 
+        else  if beq_nat n nl then mkline s1 None
+        else if beq_nat n sep then
+         match acc with 
+          Some x =>  app (rev x) (mkline s1 (Some nil))
+        | None => mkline s1 (Some nil)
+         end 
+        else if is_num n then
+         match acc with 
+          Some x =>  mkline s1 (Some  ((get_num n)::x))
+        | None => mkline s1 None
+         end  else mkline s1 None
+   | _ => nil
+  end.
+
+Definition parse p := mkline p None.
