Print.v
@@ -1,0 +1,71 @@
+(* This program is free software; you can redistribute it and/or      *)
+(* modify it under the terms of the GNU Lesser General Public License *)
+(* as published by the Free Software Foundation; either version 2.1   *)
+(* of the License, or (at your option) any later version.             *)
+(*                                                                    *)
+(* This program is distributed in the hope that it will be useful,    *)
+(* but WITHOUT ANY WARRANTY; without even the implied warranty of     *)
+(* MERCHANTABILITY or FITNESS FOR A PARTICULAR PURPOSE.  See the      *)
+(* GNU General Public License for more details.                       *)
+(*                                                                    *)
+(* You should have received a copy of the GNU Lesser General Public   *)
+(* License along with this program; if not, write to the Free         *)
+(* Software Foundation, Inc., 51 Franklin St, Fifth Floor, Boston, MA *)
+(* 02110-1301 USA                                                     *)
+
+Require Import List.
+Require Import String.
+
+(* Printing function *)
+
+Fixpoint is_eq (n m: nat) {struct n} :=
+ match n, m with 
+  0, 0 => true | (S n1), (S m1) => is_eq n1 m1 | _ ,_ => false end.
+
+Fixpoint adiv (n m p: nat) {struct p} :=
+  match p with 0 => false | (S p1) =>
+    if (is_eq n m) then true else adiv (n - m) m p1
+  end.
+
+Definition div n m := 
+match m with 0 => true | _ => adiv m n m end.
+
+Fixpoint print_line (n m: nat) (l: list nat) {struct n}: 
+  string * list nat :=
+let v := if (div m n) then "|"%string else ""%string in
+match n, l with
+    O  ,    _ => (v, l)
+|  (S n1), (0 :: l1) => 
+    let (s1, l2) := print_line n1 m l1 in
+                 (append v (append " " s1),
+                  l2)
+|  (S n1), (n :: l1) => 
+    let (s1, l2) := print_line n1 m l1 in
+                 (append v 
+                  (String (Ascii.ascii_of_nat (n + 48)) s1),
+                  l2)
+| _,_ => ("error"%string , l)
+end. 
+
+Fixpoint paux (m n p q: nat) (s: string) (l: list nat) {struct m}: 
+  string :=
+let v := if (div p m) then s else ""%string in
+append v 
+match m with
+    O      => ""%string
+|  (S m1)  =>
+    let (s1, l1) := print_line n q l in
+      append s1 (String (Ascii.ascii_of_nat 10) (paux m1 n p q s l1))
+end. 
+
+Fixpoint print_sep (n: nat): string :=
+  match n with 0 => ""%string | S n1 => append "-" (print_sep n1) end.
+
+Definition print n m s :=
+  let lf := Ascii.ascii_of_nat 10 in
+  let nm := n * m in 
+  let s1 := (append 
+               (print_sep (1 + n + nm))
+               (String lf ""%string)) 
+ in
+  String lf (paux nm nm n m s1 s).
